WIP for alice

KeyManagement/MessageEq.v
@@ -15,26 +15,37 @@
  * or 7014 (Feb 2014). Notwithstanding any copyright notice, U.S. Government rights in this work are
  * defined by DFARS 252.227-7013 or DFARS 252.227-7014 as detailed above. Use of this work other than
  *  as specifically authorized by the U.S. Government may violate any copyrights that exist in this work. *)
-Require Import ChMaps Messages Maps.
-Require RealWorld IdealWorld Common Keys MyPrelude.
 From Coq Require Import List.
 
-(* Module Foo <: EMPTY. End Foo. *)
-(* Module Import SN := SetNotations(Foo). *)
+Require Import
+        MyPrelude
+        AdversaryUniverse
+        ChMaps
+        Messages
+        Maps
+        Common
+        Keys
+        Tactics
+.
 
+Require Import MessagesTheory.
+
+Require RealWorld IdealWorld.
 Import RealWorld.RealWorldNotations.
 Import IdealWorld.IdealNotations.
 (* assumes that there is a shadow copy of the built message in every store in the cipherheap *)
 (* potential major refactor for usage/id/sym interraction?*)
 
-Fixpoint content_eq  {t__rw t__iw} (m__rw : RealWorld.message.message t__rw) (m__iw : IdealWorld.message.message t__iw) gks : Prop :=
+Fixpoint content_eq  {t__rw t__iw}
+         (m__rw : RealWorld.message.message t__rw)
+         (m__iw : IdealWorld.message.message t__iw) gks : Prop :=
   match (m__rw, m__iw) with
   | (RealWorld.message.Content c__rw, IdealWorld.message.Content c__iw) => c__rw = c__iw
-  | (RealWorld.message.Permission (id, _) , IdealWorld.message.Permission (IdealWorld.construct_access a _)) =>
+  | (RealWorld.message.Permission (id, pk) , IdealWorld.message.Permission (IdealWorld.construct_access a _)) =>
     match (gks $? id) with
     | Some (Keys.MkCryptoKey id _ Keys.SymKey) => a = (IdealWorld.construct_permission true true)
-    | Some (Keys.MkCryptoKey id Keys.Signing Keys.AsymKey) => a = (IdealWorld.construct_permission true false)
-    | Some (Keys.MkCryptoKey id Keys.Encryption Keys.AsymKey) => a = (IdealWorld.construct_permission false true)
+    | Some (Keys.MkCryptoKey id Keys.Signing Keys.AsymKey) => a = (IdealWorld.construct_permission true pk)
+    | Some (Keys.MkCryptoKey id Keys.Encryption Keys.AsymKey) => a = (IdealWorld.construct_permission pk true)
     | _ => False
     end
   | (RealWorld.message.MsgPair m__rw1 m__rw2, IdealWorld.message.MsgPair m__iw1 m__iw2) =>
@@ -52,38 +63,373 @@ Definition resolve_perm (ps : IdealWorld.permissions) id :=
     end
   end.
 
+Definition not_replayed (cs : RealWorld.ciphers) (honestk : key_perms)
+           (uid : user_id) (froms : RealWorld.recv_nonces) {t} (msg : RealWorld.crypto t) :=
+  RealWorld.msg_honestly_signed honestk cs msg
+  && RealWorld.msg_to_this_user cs (Some uid) msg
+  && match msg_nonce_ok cs froms msg with
+     | Some f => true
+     | None   => false
+     end.
+
+Definition key_perms_from_known_ciphers (cs : RealWorld.ciphers) (mycs : RealWorld.my_ciphers) (ks0 : key_perms) :=
+  fold_left (fun kys cid => match cs $? cid with
+                         | Some (RealWorld.SigCipher _ _ _ m) => kys $k++ RealWorld.findKeysMessage m
+                         | Some (RealWorld.SigEncCipher _ _ _ _ m) => kys $k++ RealWorld.findKeysMessage m
+                         | None => kys
+                         end) mycs ks0.
+
+Definition key_perms_from_message_queue (cs : RealWorld.ciphers) (honestk: key_perms)
+           (msgs : RealWorld.queued_messages) (uid : user_id) (froms : RealWorld.recv_nonces) (ks0 : key_perms) :=
+  let cmsgs := clean_messages honestk cs (Some uid) froms msgs
+  in  fold_left (fun kys '(existT _ _ m) => kys $k++ RealWorld.findKeysCrypto cs m) cmsgs.
+
+
+(* Definition key_perms_from_message_queue (cs : RealWorld.ciphers) (honestk: key_perms) *)
+(*            (msgs : RealWorld.queued_messages) (uid : user_id) (froms : RealWorld.recv_nonces) (ks0 : key_perms) := *)
+(*   match msgs with *)
+(*   | (existT _ _ m :: ms) => if not_replayed cs honestk uid froms m *)
+(*                           then ks0 $k++ RealWorld.findKeysCrypto cs m *)
+(*                           else ks0 *)
+(*   | _                   => ks0 *)
+(*   end. *)
+
+Lemma key_perms_from_known_ciphers_notation :
+  forall cs mycs ks,
+  fold_left (fun kys cid => match cs $? cid with
+                         | Some (RealWorld.SigCipher _ _ _ m) => kys $k++ RealWorld.findKeysMessage m
+                         | Some (RealWorld.SigEncCipher _ _ _ _ m) => kys $k++ RealWorld.findKeysMessage m
+                         | None => kys
+                         end) mycs ks
+  = key_perms_from_known_ciphers cs mycs ks.
+  unfold key_perms_from_known_ciphers; trivial.
+Qed.
+
+Lemma key_perms_from_message_queue_notation :
+  forall cs honestk msgs ks uid froms,
+    (let cmsgs := clean_messages honestk cs (Some uid) froms msgs
+     in  fold_left (fun kys '(existT _ _ m) => kys $k++ RealWorld.findKeysCrypto cs m) cmsgs)
+    = key_perms_from_message_queue cs honestk msgs uid froms ks.
+  unfold key_perms_from_message_queue; trivial.
+Qed.
+
+Lemma clean_messages_cons_split :
+  forall cs honestk uid froms msgs cmsgs t (msg : RealWorld.crypto t),
+    cmsgs = clean_messages honestk cs (Some uid) froms ((existT _ _ msg) :: msgs)
+    -> (cmsgs = clean_messages honestk cs (Some uid) froms msgs /\ not_replayed cs honestk uid froms msg = false)
+      \/ exists n, 
+        cmsgs = (existT _ _ msg) :: clean_messages honestk cs (Some uid) (n :: froms) msgs
+        /\ not_replayed cs honestk uid froms msg = true.
+Proof.
+  unfold clean_messages, clean_messages'; simpl; intros.
+  cases (not_replayed cs honestk uid froms msg); subst; simpl;
+    unfold not_replayed in * |- ; unfold RealWorld.msg_signed_addressed.
+
+  - right.
+    rewrite !andb_true_iff in *; split_ex.
+    rewrite H, H1; simpl.
+    unfold msg_nonce_ok in *; destruct msg; try discriminate.
+    cases (cs $? c_id); try discriminate.
+    cases (count_occ RealWorld.msg_seq_eq froms (RealWorld.cipher_nonce c)); try discriminate.
+    eexists; split; eauto.
+    rewrite !fold_clean_messages2', clean_messages'_fst_pull, !fold_clean_messages; simpl; trivial.
+
+  - left.
+    cases (RealWorld.msg_honestly_signed honestk cs msg); eauto.
+    cases (RealWorld.msg_to_this_user cs (Some uid) msg); eauto.
+    simpl.
+    cases (msg_nonce_ok cs froms msg); try discriminate; eauto.
+Qed.
+
+Lemma key_perms_from_known_ciphers_pull_merge :
+  forall cs mycs ks newk,
+    key_perms_from_known_ciphers cs mycs (ks $k++ newk)
+    = key_perms_from_known_ciphers cs mycs ks $k++ newk.
+Proof.
+  unfold key_perms_from_known_ciphers.
+  induction mycs; intros; eauto.
+  simpl.
+  cases (cs $? a); eauto.
+  destruct c; eauto.
+  - rewrite merge_perms_assoc, merge_perms_sym with (ks1 := newk), <- merge_perms_assoc.
+    specialize (IHmycs (ks $k++ RealWorld.findKeysMessage msg) newk); eauto.
+  - rewrite merge_perms_assoc, merge_perms_sym with (ks1 := newk), <- merge_perms_assoc.
+    specialize (IHmycs (ks $k++ RealWorld.findKeysMessage msg) newk); eauto.
+Qed.
+
+Lemma key_perms_from_message_queue_pull_merge :
+  forall cs msgs ks honestk uid froms newk,
+    key_perms_from_message_queue' cs honestk msgs uid froms (ks $k++ newk)
+    = key_perms_from_message_queue' cs honestk msgs uid froms ks $k++ newk.
+Proof.
+  unfold key_perms_from_message_queue'.
+  induction msgs; intros; eauto.
+  simpl; destruct a.
+  cases (not_replayed cs honestk uid froms c); eauto.
+
+  rewrite merge_perms_assoc, merge_perms_sym with (ks1 := newk), <- merge_perms_assoc; trivial.
+Qed.
+
+Lemma key_perms_from_known_ciphers_idempotent_add_known_cipher :
+  forall cs mycs ks c_id c newk,
+    cs $? c_id = Some c
+    -> List.In c_id mycs
+    -> newk = match c with
+             | (RealWorld.SigCipher _ _ _ m) => RealWorld.findKeysMessage m
+             | (RealWorld.SigEncCipher _ _ _ _ m) => RealWorld.findKeysMessage m
+             end
+    -> key_perms_from_known_ciphers cs mycs ks
+      = key_perms_from_known_ciphers cs mycs (ks $k++ newk).
+Proof.
+  induction mycs; intros; eauto.
+  invert H0.
+
+  invert H0.
+  - simpl; context_map_rewrites.
+    destruct c; eauto.
+    symmetry; rewrite merge_perms_assoc, merge_perms_refl; trivial.
+    symmetry; rewrite merge_perms_assoc, merge_perms_refl; trivial.
+    
+  - eapply IHmycs with (ks := ks) in H2; eauto.
+    simpl.
+    cases (cs $? a); eauto.
+    destruct c, c0; eauto.
+
+    all :
+      symmetry; rewrite key_perms_from_known_ciphers_pull_merge;
+      symmetry; rewrite key_perms_from_known_ciphers_pull_merge, <- H2; trivial.
+Qed.
+
+Lemma key_perms_from_message_queue_idempotent_add_known_message :
+  forall t (msg : RealWorld.crypto t) msgs cs honestk ks uid froms newk,
+    List.In (existT _ _ msg) msgs
+    -> newk = (if not_replayed cs honestk uid froms msg
+              then RealWorld.findKeysCrypto cs msg
+              else $0)
+    -> key_perms_from_message_queue' cs honestk msgs uid froms ks
+      = key_perms_from_message_queue' cs honestk msgs uid froms (ks $k++ newk).
+Proof.
+  induction msgs; intros; eauto.
+  invert H.
+
+  invert H; simpl.
+  - cases ( not_replayed cs honestk uid froms msg ); eauto.
+    symmetry; rewrite merge_perms_assoc, merge_perms_refl; trivial.
+    
+  - eapply IHmsgs with (ks := ks) (cs := cs) (honestk := honestk) in H1; eauto.
+    destruct a; simpl in *.
+    cases ( not_replayed cs honestk uid froms c ); eauto.
+    cases ( not_replayed cs honestk uid froms msg ); eauto.
+
+    rewrite key_perms_from_message_queue_pull_merge.
+    symmetry; rewrite key_perms_from_message_queue_pull_merge.
+    rewrite <- H1; trivial.
+Qed.
+
+Inductive user_perms_channel_match {A} (uid : user_id) (usr__rw : RealWorld.user_data A) (usr__iw : IdealWorld.user A)
+          (honestk : key_perms) (cs : RealWorld.ciphers) (c_id : RealWorld.cipher_id) (ch_id : channel_id) : Prop :=
+
+| SigChannel : forall mks cks ks b__read b__write k__sign u_id msg_seq t (m__rw : RealWorld.message.message t),
+    RealWorld.honest_key honestk k__sign
+    -> cs $? c_id = Some (RealWorld.SigCipher k__sign u_id msg_seq m__rw)
+    -> cks = key_perms_from_known_ciphers cs usr__rw.(RealWorld.c_heap) $0
+    -> mks = key_perms_from_message_queue cs honestk usr__rw.(RealWorld.msg_heap) uid usr__rw.(RealWorld.from_nons) $0
+    -> ks = usr__rw.(RealWorld.key_heap) $k++ cks $k++ mks
+    -> resolve_perm usr__iw.(IdealWorld.perms) ch_id = Some (IdealWorld.construct_permission b__read b__write)
+    (* -> ks $? k__sign = None *)
+    -> ks $? k__sign = Some b__write
+    -> b__read = true
+    -> user_perms_channel_match uid usr__rw usr__iw honestk cs c_id ch_id
+| SigEncChannel : forall mks cks ks b__read b__write k__sign k__enc u_id msg_seq t (m__rw : RealWorld.message.message t),
+    RealWorld.honest_key honestk k__sign
+    -> cs $? c_id = Some (RealWorld.SigEncCipher k__sign k__enc u_id msg_seq m__rw)
+    -> cks = key_perms_from_known_ciphers cs usr__rw.(RealWorld.c_heap) $0
+    -> mks = key_perms_from_message_queue cs honestk usr__rw.(RealWorld.msg_heap) uid usr__rw.(RealWorld.from_nons) $0
+    -> ks = usr__rw.(RealWorld.key_heap) $k++ cks $k++ mks
+    -> resolve_perm usr__iw.(IdealWorld.perms) ch_id = Some (IdealWorld.construct_permission b__read b__write)
+    (* -> ( ks $? k__sign = None \/ ks $? k__enc = None ) *)
+    -> ks $? k__sign = Some b__write
+    -> ks $? k__enc  = Some b__read
+    -> user_perms_channel_match uid usr__rw usr__iw honestk cs c_id ch_id
+.
+
+Lemma ch_keys_from_cipher :
+  forall A (usr usr' : RealWorld.user_data A) usr__iw honestk uid cs c_id c_id' c ch_id newk,
+    cs $? c_id' = Some c
+    (* -> c_id <> c_id' *)
+    -> List.In c_id' usr.(RealWorld.c_heap)
+    -> newk = match c with
+             | (RealWorld.SigCipher _ _ _ m) => RealWorld.findKeysMessage m
+             | (RealWorld.SigEncCipher _ _ _ _ m) => RealWorld.findKeysMessage m
+             end
+    -> usr' = RealWorld.addUserKeys newk usr
+    -> user_perms_channel_match uid usr usr__iw honestk cs c_id ch_id
+    -> user_perms_channel_match uid usr' usr__iw honestk cs c_id ch_id.
+Proof.
+  intros.
+  invert H3; [ econstructor 1 | econstructor 2]; simpl; eauto.
+
+  all : 
+    rewrite merge_perms_assoc with (ks3 := key_perms_from_known_ciphers cs (RealWorld.c_heap usr) $0);
+    rewrite merge_perms_sym with (ks2 := key_perms_from_known_ciphers cs (RealWorld.c_heap usr) $0);
+    rewrite <- key_perms_from_known_ciphers_pull_merge;
+    erewrite <- key_perms_from_known_ciphers_idempotent_add_known_cipher with (c_id := c_id'); eauto.
+Qed.
+
+Lemma ch_keys_from_cipher_inv :
+  forall A (usr usr' : RealWorld.user_data A) usr__iw honestk cs uid c_id c_id' c ch_id newk,
+    cs $? c_id' = Some c
+    (* -> c_id <> c_id' *)
+    -> List.In c_id' usr.(RealWorld.c_heap)
+    -> newk = match c with
+             | (RealWorld.SigCipher _ _ _ m) => RealWorld.findKeysMessage m
+             | (RealWorld.SigEncCipher _ _ _ _ m) => RealWorld.findKeysMessage m
+             end
+    -> usr' = RealWorld.addUserKeys newk usr
+    -> user_perms_channel_match uid usr' usr__iw honestk cs c_id ch_id
+    -> user_perms_channel_match uid usr usr__iw honestk cs c_id ch_id.
+Proof.
+  intros.
+  invert H3; [ econstructor 1 | econstructor 2]; simpl in *; eauto; simpl in *.
+
+  all : 
+    rewrite merge_perms_assoc with (ks3 := key_perms_from_known_ciphers cs (RealWorld.c_heap usr) $0) in H10;
+    rewrite merge_perms_sym with (ks2 := key_perms_from_known_ciphers cs (RealWorld.c_heap usr) $0) in H10;
+    rewrite <- key_perms_from_known_ciphers_pull_merge in H10;
+    erewrite <- key_perms_from_known_ciphers_idempotent_add_known_cipher with (c_id := c_id') in H10; eauto.
+
+  rewrite merge_perms_assoc with (ks3 := key_perms_from_known_ciphers cs (RealWorld.c_heap usr) $0) in H11;
+    rewrite merge_perms_sym with (ks2 := key_perms_from_known_ciphers cs (RealWorld.c_heap usr) $0) in H11;
+    rewrite <- key_perms_from_known_ciphers_pull_merge in H11;
+    erewrite <- key_perms_from_known_ciphers_idempotent_add_known_cipher with (c_id := c_id') in H11; eauto.
+Qed.
+
+(* Lemma ch_keys_from_msg : *)
+(*   forall A (usr usr' : RealWorld.user_data A) t (msg : RealWorld.crypto t) usr__iw cs honestk newk uid c_id ch_id, *)
+(*     List.In (existT _ _ msg) usr.(RealWorld.msg_heap) *)
+(*     -> newk = (if RealWorld.msg_honestly_signed honestk cs msg *)
+(*               then RealWorld.findKeysCrypto cs msg *)
+(*               else $0) *)
+(*     -> usr' = {| RealWorld.key_heap  := usr.(RealWorld.key_heap) *)
+(*                 ; RealWorld.protocol  := usr.(RealWorld.protocol) *)
+(*                 ; RealWorld.msg_heap  := (existT _ _ msg) :: usr.(RealWorld.msg_heap) *)
+(*                 ; RealWorld.c_heap    := usr.(RealWorld.c_heap) *)
+(*                 ; RealWorld.from_nons := usr.(RealWorld.from_nons) *)
+(*                 ; RealWorld.sent_nons := usr.(RealWorld.sent_nons) *)
+(*                 ; RealWorld.cur_nonce := usr.(RealWorld.cur_nonce) *)
+(*              |} *)
+(*     -> user_perms_channel_match uid usr usr__iw honestk cs c_id ch_id *)
+(*     -> user_perms_channel_match uid usr' usr__iw honestk cs c_id ch_id. *)
+(* Proof. *)
+(*   intros. *)
+(*   invert H2; [ econstructor 1 | econstructor 2]; simpl; eauto; *)
+(*     cases (not_replayed cs honestk uid usr.(RealWorld.from_nons) msg); eauto. *)
+
+(*   all :  *)
+(*     erewrite <- key_perms_from_message_queue_idempotent_add_known_message; eauto; rewrite Heq; eauto. *)
+(* Qed. *)
+
+(* Lemma ch_keys_from_msg_inv : *)
+(*   forall A (usr usr' : RealWorld.user_data A) t (msg : RealWorld.crypto t) usr__iw cs honestk newk uid c_id ch_id, *)
+(*     List.In (existT _ _ msg) usr.(RealWorld.msg_heap) *)
+(*     -> newk = (if RealWorld.msg_honestly_signed honestk cs msg *)
+(*               then RealWorld.findKeysCrypto cs msg *)
+(*               else $0) *)
+(*     -> usr' = {| RealWorld.key_heap  := usr.(RealWorld.key_heap) *)
+(*                 ; RealWorld.protocol  := usr.(RealWorld.protocol) *)
+(*                 ; RealWorld.msg_heap  := (existT _ _ msg) :: usr.(RealWorld.msg_heap) *)
+(*                 ; RealWorld.c_heap    := usr.(RealWorld.c_heap) *)
+(*                 ; RealWorld.from_nons := usr.(RealWorld.from_nons) *)
+(*                 ; RealWorld.sent_nons := usr.(RealWorld.sent_nons) *)
+(*                 ; RealWorld.cur_nonce := usr.(RealWorld.cur_nonce) *)
+(*              |} *)
+(*     -> user_perms_channel_match uid usr' usr__iw honestk cs c_id ch_id *)
+(*     -> user_perms_channel_match uid usr usr__iw honestk cs c_id ch_id. *)
+(* Proof. *)
+(*   intros. *)
+(*   invert H2; [ econstructor 1 | econstructor 2]; simpl; eauto; simpl in *; *)
+(*     cases (not_replayed cs honestk uid usr.(RealWorld.from_nons) msg); eauto. *)
+
+(*   erewrite <- key_perms_from_message_queue_idempotent_add_known_message in H9; eauto; rewrite Heq; trivial. *)
+(*   erewrite <- key_perms_from_message_queue_idempotent_add_known_message in H9; eauto; rewrite Heq; trivial. *)
+(*   erewrite <- key_perms_from_message_queue_idempotent_add_known_message in H10; eauto; rewrite Heq; trivial. *)
+(* Qed. *)
+
 Inductive  message_eq : forall {A B t},
-  RealWorld.crypto t -> RealWorld.universe A B ->
-  IdealWorld.message.message t -> IdealWorld.universe A -> IdealWorld.channel_id -> Prop :=
-| ContentCase : forall {A B t}  (U__rw : RealWorld.universe A B) U__iw (m__rw : RealWorld.message.message t) m__iw ch_id user_data,
-    content_eq m__rw m__iw U__rw.(RealWorld.all_keys)
-    -> (forall u, U__iw.(IdealWorld.users) $? u  = Some user_data
-            -> resolve_perm user_data.(IdealWorld.perms) ch_id = Some (IdealWorld.construct_permission true true))
-    -> message_eq (RealWorld.Content m__rw) U__rw m__iw U__iw ch_id
+    RealWorld.crypto t -> RealWorld.universe A B ->
+    IdealWorld.message.message t -> IdealWorld.universe A -> IdealWorld.channel_id -> Prop :=
 | CryptoSigCase : forall {A B t} (U__rw : RealWorld.universe A B) U__iw (m__iw : IdealWorld.message.message t) c_id ch_id k__sign
-                    (m__rw : RealWorld.message.message t) b__iw honestk u_id msg_seq,
+                    (m__rw : RealWorld.message.message t) honestk u_id msg_seq,
     U__rw.(RealWorld.all_ciphers) $? c_id = Some (RealWorld.SigCipher k__sign u_id msg_seq m__rw)
     -> content_eq m__rw m__iw U__rw.(RealWorld.all_keys)
     -> honestk = RealWorld.findUserKeys (U__rw.(RealWorld.users))
     -> (forall u data__rw data__iw,
-	                     U__rw.(RealWorld.users) $? u = Some data__rw
-                          -> U__iw.(IdealWorld.users) $? u = Some data__iw
-                          ->  RealWorld.honest_key honestk k__sign
-          (*sign key is honest.  honest key : find user keys on all users*)
-            -> (data__rw.(RealWorld.key_heap) $? k__sign = Some true
-               -> resolve_perm data__iw.(IdealWorld.perms) ch_id = Some (IdealWorld.construct_permission true b__iw)))
+	  U__rw.(RealWorld.users) $? u = Some data__rw
+          -> U__iw.(IdealWorld.users) $? u = Some data__iw
+          -> RealWorld.honest_key honestk k__sign
+          -> user_perms_channel_match u data__rw data__iw honestk U__rw.(RealWorld.all_ciphers) c_id ch_id)
+    (* -> (forall u data__rw data__iw b__read b__write, *)
+    (*       U__rw.(RealWorld.users) $? u = Some data__rw *)
+    (*       -> U__iw.(IdealWorld.users) $? u = Some data__iw *)
+    (*       -> RealWorld.honest_key honestk k__sign *)
+    (*       -> resolve_perm data__iw.(IdealWorld.perms) ch_id = Some (IdealWorld.construct_permission b__read b__write) *)
+    (*       -> data__rw.(RealWorld.key_heap) $? k__sign = None *)
+    (*       \/ (data__rw.(RealWorld.key_heap) $? k__sign = Some b__write /\ b__read = true) *)
+    (*   ) *)
     -> message_eq (RealWorld.SignedCiphertext c_id) U__rw m__iw U__iw ch_id
+
 | CryptoSigEncCase : forall {A B t} (U__rw : RealWorld.universe A B) U__iw (m__iw : IdealWorld.message.message t) c_id ch_id k__sign k__enc
                        (m__rw : RealWorld.message.message t) honestk u_id msg_seq,
     U__rw.(RealWorld.all_ciphers) $? c_id = Some (RealWorld.SigEncCipher k__sign k__enc u_id msg_seq m__rw)
     -> content_eq m__rw m__iw U__rw.(RealWorld.all_keys)
-    -> honestk = RealWorld.findUserKeys (U__rw.(RealWorld.users))
-    -> (forall u data__rw data__iw b__rwenc,
-	                     U__rw.(RealWorld.users) $? u = Some data__rw
-                          -> U__iw.(IdealWorld.users) $? u = Some data__iw
-                          -> RealWorld.honest_key honestk k__sign
-                          -> RealWorld.honest_key honestk k__enc
-            -> ((data__rw.(RealWorld.key_heap) $? k__sign = Some true
-                /\ data__rw.(RealWorld.key_heap) $? k__enc = Some b__rwenc)
-               -> resolve_perm data__iw.(IdealWorld.perms) ch_id = Some (IdealWorld.construct_permission b__rwenc true)))
+    -> honestk = RealWorld.findUserKeys U__rw.(RealWorld.users)
+    -> (forall u data__rw data__iw,
+	  U__rw.(RealWorld.users) $? u = Some data__rw
+          -> U__iw.(IdealWorld.users) $? u = Some data__iw
+          -> RealWorld.honest_key honestk k__sign
+          -> RealWorld.honest_key honestk k__enc
+          -> user_perms_channel_match u data__rw data__iw honestk U__rw.(RealWorld.all_ciphers) c_id ch_id
+          (* -> resolve_perm data__iw.(IdealWorld.perms) ch_id = Some (IdealWorld.construct_permission b__read b__write) *)
+          (* -> ( data__rw.(RealWorld.key_heap) $? k__sign = None \/ data__rw.(RealWorld.key_heap) $? k__enc = None ) *)
+          (* \/ ( data__rw.(RealWorld.key_heap) $? k__sign = Some b__write *)
+          (*   /\ data__rw.(RealWorld.key_heap) $? k__enc  = Some b__read) *)
+      )
     -> message_eq (RealWorld.SignedCiphertext c_id) U__rw m__iw U__iw ch_id.
+
+
+(* Inductive  message_eq : forall {A B t}, *)
+(*     RealWorld.crypto t -> RealWorld.universe A B -> *)
+(*     IdealWorld.message.message t -> IdealWorld.universe A -> IdealWorld.channel_id -> Prop := *)
+(* | ContentCase : *)
+(*     forall {A B t} (U__rw : RealWorld.universe A B) U__iw (m__rw : RealWorld.message.message t) m__iw ch_id user_data, *)
+(*       content_eq m__rw m__iw U__rw.(RealWorld.all_keys) *)
+(*     -> (forall u, U__iw.(IdealWorld.users) $? u  = Some user_data *)
+(*             -> resolve_perm user_data.(IdealWorld.perms) ch_id = Some (IdealWorld.construct_permission true true)) *)
+(*     -> message_eq (RealWorld.Content m__rw) U__rw m__iw U__iw ch_id *)
+(* | CryptoSigCase : forall {A B t} (U__rw : RealWorld.universe A B) U__iw (m__iw : IdealWorld.message.message t) c_id ch_id k__sign *)
+(*                     (m__rw : RealWorld.message.message t) b__iw honestk u_id msg_seq, *)
+(*     U__rw.(RealWorld.all_ciphers) $? c_id = Some (RealWorld.SigCipher k__sign u_id msg_seq m__rw) *)
+(*     -> content_eq m__rw m__iw U__rw.(RealWorld.all_keys) *)
+(*     -> honestk = RealWorld.findUserKeys (U__rw.(RealWorld.users)) *)
+(*     -> (forall u data__rw data__iw, *)
+(* 	  U__rw.(RealWorld.users) $? u = Some data__rw *)
+(*           -> U__iw.(IdealWorld.users) $? u = Some data__iw *)
+(*           ->  RealWorld.honest_key honestk k__sign *)
+(*           (*sign key is honest.  honest key : find user keys on all users*) *)
+(*           -> (data__rw.(RealWorld.key_heap) $? k__sign = Some true *)
+(*              -> resolve_perm data__iw.(IdealWorld.perms) ch_id = Some (IdealWorld.construct_permission true b__iw))) *)
+(*     -> message_eq (RealWorld.SignedCiphertext c_id) U__rw m__iw U__iw ch_id *)
+(* | CryptoSigEncCase : forall {A B t} (U__rw : RealWorld.universe A B) U__iw (m__iw : IdealWorld.message.message t) c_id ch_id k__sign k__enc *)
+(*                        (m__rw : RealWorld.message.message t) honestk u_id msg_seq, *)
+(*     U__rw.(RealWorld.all_ciphers) $? c_id = Some (RealWorld.SigEncCipher k__sign k__enc u_id msg_seq m__rw) *)
+(*     -> content_eq m__rw m__iw U__rw.(RealWorld.all_keys) *)
+(*     -> honestk = RealWorld.findUserKeys (U__rw.(RealWorld.users)) *)
+(*     -> (forall u data__rw data__iw b__rwenc, *)
+(* 	  U__rw.(RealWorld.users) $? u = Some data__rw *)
+(*           -> U__iw.(IdealWorld.users) $? u = Some data__iw *)
+(*           -> RealWorld.honest_key honestk k__sign *)
+(*           -> RealWorld.honest_key honestk k__enc *)
+(*           -> ((data__rw.(RealWorld.key_heap) $? k__sign = Some true *)
+(*               /\ data__rw.(RealWorld.key_heap) $? k__enc = Some b__rwenc) *)
+(*              -> resolve_perm data__iw.(IdealWorld.perms) ch_id = Some (IdealWorld.construct_permission b__rwenc true))) *)
+(*     -> message_eq (RealWorld.SignedCiphertext c_id) U__rw m__iw U__iw ch_id. *)
