KeyManagement/Automation.v
@@ -26,7 +26,7 @@ Require Import
         Common
         Maps
         Keys
-        Messages
+        (* Messages *)
         RealWorld
         Simulation.
 
